in the middle of Handshake.fst

src/tls/Handshake.fst
@@ -8,6 +8,7 @@ open FStar.HyperHeap
 open FStar.HyperStack
 //FIXME! Don't open so much ... gets confusing. Use module abbrevs instead
 //AR: Yes ! Totally agree.
+//CF: TODO.
 open FStar.Seq
  // for e.g. found
 open FStar.Set
@@ -38,90 +39,15 @@ module Nego = Negotiation
 
 let hashSize = Hashing.Spec.tagLen
 
-//<expose for TestClient>
-#set-options "--lax"
+//<expose for TestClient> CF: temporarily broken; such tests should be coded against HS submodules.
+// TODO restore unit tests as in TestClient
 
 (* A flag for runtime debugging of Handshake data.
    The F* normalizer will erase debug prints at extraction
    when this flag is set to false. *)
 inline_for_extraction let hs_debug = false
 
-(* Sketch 
-val Nego.prepareClientOffer: config -> clientOffer
-let Nego.prepareClientOffer cfg =
-  let groups = List.Tot.choose CommonDH.group_of_namedGroup cfg.namedGroups in
-  let cipher_suites = ... in
-  let sigAlgs = ... in
-  let protocol_version = ... in
-  let ext = prepareExtensions protocol_version cipher_suites sigAlgs groups kp in
-*)  
 
-
-val prepareClientHello: 
-  st:hs {st.role = Client}
-  -> ST hs_msg
-  (requires (fun h -> True)) //TODO: add the precondition that Nego and KS are in proper state
-  (ensures (fun h0 i h1 -> True))
-  (* TODO: what should we say here? something like:
-    - The Keys Schedule state machine is in the initial state
-    - The Handshake log has exactly one more message: the ClientHello computed from the input configurtion
-    - The result is this ClientHello and its serialization
-  *)
-let prepareClientHello st = 
-  (* Negotiation computes the list of groups from the configuration;
-     KeySchedule computes and serializes the shares from these groups (calling into CommonDH)
-     Messages should do the serialization (calling into CommonDH), but dependencies are tricky
-  *)
-  (* In Negotiation: compute offer from configuration *)
-  let offer = Nego.prepareClientOffer hs.nego hs.cfg hs.resume in
-  (* In KeySchedule: compute shares for groups in offer *)
-  let shares =
-    match offer.co_protocol_version with
-    | TLS_1p3 -> Some (KeySchedule.ks_client_13_1rtt_init hs.ks offer.co_namedGroups)
-    | _       -> let si = KeySchedule.ks_client_12_init ks in None
-    in
-  (* Some? sido in case of resumption *)
-  let sid =
-    match fst hs.resume with
-    | None -> empty_bytes
-    | Some x -> x
-  in
-  (* In TLSExtensions: prepare client extensions, including key shares *)
-  let ext = prepareExtensions offer hs.resume ri shares in
-  let ch = // a bit too concrete? ClientHello hs.nonce offer hs.resume ri shares
-  {
-    ch_protocol_version = offer.co_protocol_version;
-    ch_client_random = hs.nonce;
-    ch_sessionID = sid;
-    ch_cipher_suites = offer.co_cipher_suites;
-    ch_raw_cipher_suites = None;
-    ch_compressions = offer.co_compressions;
-    ch_extensions = Some ext
-  } in
-  HandshakeLog.send hs.log (ClientHello ch) in
-  // TODO in two steps, appending the binders
-  ClientHello ch
-
-
-(*
-//16-05-31 somewhat duplicating TLSConstants.geqPV
-(* Is [pv1 >= pv2]? *)
-val gte_pv: protocolVersion -> protocolVersion -> Tot bool
-let gte_pv pv1 pv2 =
-  match pv1 with
-  | SSL_3p0 -> (match pv2 with | SSL_3p0 -> true | _ -> false)
-  | TLS_1p0 -> (match pv2 with | SSL_3p0 | TLS_1p0 -> true | _ -> false)
-  | TLS_1p1 -> (match pv2 with | SSL_3p0 | TLS_1p0 | TLS_1p1 -> true | _ -> false)
-  | TLS_1p2 -> (match pv2 with | TLS_1p3 -> false | _ -> true)
-  | TLS_1p3 -> true
-
-//SZ: Indeed.
-val gte_pv_geqPV: pv1:protocolVersion -> pv2:protocolVersion
-  -> Lemma (gte_pv pv1 pv2 <==> geqPV pv1 pv2)
-let gte_pv_geqPV pv1 pv2 = ()
-*)
-
-#reset-options
 
 (* Returns [c] if [c] is within the range of acceptable versions for [cfg],
  * [Error] otherwise. *)
@@ -132,120 +58,13 @@ val getCachedSession: cfg:config -> ch:ch -> ST (option session)
   (ensures (fun h0 i h1 -> True))
 let getCachedSession cfg cg = None
 
-#set-options "--lax"
-
-// FIXME: TLS1.3
-// no point sharing between TLS 1.2 and TLS 1.3?
-val prepareServerHello: 
-  st: hs {st.role = Server} -> 
-  // config -> 
-  // KeySchedule.ks -> 
-  // HandshakeLog.log -> 
-  // option ri -> 
-  // (hs_msg * bytes) -> 
-  ST (result (nego * option KeySchedule.recordInstance * (hs_msg * bytes)))
-  (requires (fun h -> True))
-  (ensures (fun h0 i h1 -> True))
-let prepareServerHello hs (* cfg ks log ri (ClientHello ch,_) *) =
- let negotiated = Nego.computeServerMode hs.nego hs.cfg  (* ch.ch_protocol_version ch.ch_cipher_suites ch.ch_extensions ch.ch_compressions *) hs.resume in
-  match negotiated with
-   | Error z -> Error z
-   | Correct mode ->
-     let srand = KS.ks_server_random ks in
-     let ksl =
-       (match mode.sm_protocol_version, mode.sm_dh_group, mode.sm_dh_share with
-       | TLS_1p3, Some gn, Some gxb ->
-         (match CommonDH.group_of_namedGroup gn with
-         | None -> None
-         | Some g ->
-           (match CommonDH.parse g gxb with
-           | None -> None
-           | Some gx ->
-             Some (KeySchedule.ks_server_13_1rtt_init ks ch.ch_client_random mode.sm_cipher_suite g gx)))
-       | _ -> None) in
-    (* TLSExtensions:negotiateServerExtensions *)
-    match negotiateServerExtensions mode.sm_protocol_version ch.ch_extensions ch.ch_cipher_suites cfg mode.sm_cipher_suite ri ksl false with
-    | Error(z) -> Error(z)
-    | Correct(sext) ->
-      let sid = CoreCrypto.random 32 in
-      let sh =
-      {sh_protocol_version = mode.sm_protocol_version;
-       sh_sessionID = Some sid;
-       sh_server_random = srand;
-       sh_cipher_suite = mode.sm_cipher_suite;
-       sh_compression = mode.sm_comp;
-       sh_extensions = sext} in
-      let nego =
-      {n_client_random = ch.ch_client_random;
-       n_server_random = srand;
-       n_sessionID = Some sid;
-       n_protocol_version = mode.sm_protocol_version;
-       n_kexAlg = mode.sm_kexAlg;
-       n_sigAlg = mode.sm_sigAlg;
-       n_aeAlg  = mode.sm_aeAlg;
-       n_cipher_suite = mode.sm_cipher_suite;
-       n_compression = mode.sm_comp;
-       n_dh_group = mode.sm_dh_group;
-       n_scsv = [];
-       n_extensions = mode.sm_ext;
-       (* [getCachedSession] returned [None], so no session resumption *)
-       n_resume = false} in
-       let _ = log @@ (ClientHello ch) in
-       let shb = log @@ (ServerHello sh) in
-       let keys = (match mode.sm_protocol_version with
-               | TLS_1p3 ->
-             let keys = KeySchedule.ks_server_13_sh ks in
-             Some keys
-           | _ -> None) in
-             Correct (nego,keys,(ServerHello sh,shb))
-
-val processServerHello:  // mostly Nego stuff?!
-  st:hs {st.role = Client} ->
-  // c:config -> 
-  // KeySchedule.ks -> 
-  // HandshakeLog.log -> 
-  // option ri -> 
-  ch -> 
-  (hs_msg * bytes) ->
-  ST (result (nego * option KeySchedule.recordInstance))
-     (requires (fun h -> True))
-     (ensures (fun h0 i h1 -> True))
-let processServerHello hs (* cfg ks log ri ch (ServerHello sh,_) *) =
-  let _ = log @@ (ServerHello sh) in
-  let mode = computeClientMode cfg ch.ch_extensions ch.ch_protocol_version sh.sh_protocol_version sh.sh_server_random sh.sh_cipher_suite sh.sh_extensions sh.sh_compression ri in
-   match mode with
-    | Error(z) -> Error(z)
-    | Correct(mode) ->
-   let o_nego =
-    {n_client_random = ch.ch_client_random;
-     n_server_random = sh.sh_server_random;
-     n_sessionID = sh.sh_sessionID;
-     n_protocol_version = mode.cm_protocol_version;
-     n_kexAlg = mode.cm_kexAlg;
-     n_aeAlg = mode.cm_aeAlg;
-     n_sigAlg = mode.cm_sigAlg;
-     n_cipher_suite = mode.cm_cipher_suite;
-     n_dh_group = mode.cm_dh_group;
-     n_compression = sh.sh_compression;
-     n_scsv = [];
-     n_extensions = mode.cm_ext;
-     n_resume = false } in
-    (match o_nego.n_protocol_version, o_nego.n_kexAlg, mode.cm_dh_group, mode.cm_dh_share with
-     | TLS_1p3, Kex_DHE, Some gn, Some gyb
-     | TLS_1p3, Kex_ECDHE, Some gn, Some gyb ->
-       (match CommonDH.group_of_namedGroup gn with
-       | None -> Error(AD_internal_error, perror __SOURCE_FILE__ __LINE__ "Unsupported group negotiated")
-       | Some g ->
-         (match CommonDH.parse g gyb with
-         | None -> Error(AD_decode_error, perror __SOURCE_FILE__ __LINE__ "Failed to parse server share")
-         | Some gy ->
-           let keys = KeySchedule.ks_client_13_sh ks o_nego.n_cipher_suite g gy false in
-           Correct (o_nego, Some keys)))
-     | _ -> Correct (o_nego,None))
 
 (* Handshake API: TYPES, taken from FSTI *)
 
-type clientState =
+//17-03-24 consider using instead "if role = Client then clientState else serverServer"
+//17-03-24 but that may break extraction to Kremlin and complicate typechecking
+//17-03-24 we could also use two refinements. 
+type machineState =
   | C_Idle:                  option ri -> clientState
   | C_HelloSent:       option ri -> ch -> clientState
   | C_HelloReceived:              nego -> clientState
@@ -256,11 +75,10 @@ type clientState =
   | C_Error:                     error -> clientState
   | C_PostHS:                             clientState
 
-type serverState =
   | S_Idle:                  option ri -> serverState
   | S_HelloSent :                 nego -> serverState
   | S_HelloDone :                 nego -> serverState
-  | S_CCSReceived :               nego -> serverState
+  | S_CCSReceived :               nego -> cVerifyData -> serverState
   | S_OutCCS:                     nego -> serverState
   | S_FinishedSent :              nego -> serverState
   | S_FinishedReceived :          nego -> serverState
@@ -268,16 +86,13 @@ type serverState =
   | S_ZeroRTTReceived :           nego -> serverState
   | S_Error:                     error -> serverState
   | S_PostHS:                             serverState
-
-type role_state =
-    | C of clientState
-    | S of serverState
+// TODO: review all their parameters
 
 
+// MOVE to HandshakeMessage
 //16-06-01 we don't need to precisely track this part of the state
 //16-06-01 later, pre-allocate large-enough buffers for the connection.
 //16-06-01 also revisit type of encrypted messages
-
 type hs_msg_bufs = {
      hs_incoming_parsed : list (hs_msg * bytes); // messages parsed earlier
      hs_incoming: bytes;                         // incomplete message received earlier
@@ -306,16 +121,17 @@ type resume_info (r:role) =
 type hs =
   | HS: #region: rgn { is_hs_rgn region } ->
           r: role ->
-          resume: resume_info r (* client dyn. config, both for 1.2 and 1.3 *) ->
-          cfg: config ->
           nonce: TLSInfo.random ->  // unique for all honest instances; locally enforced
+          // now both part of immutable nego state
+          // resume: resume_info r (* client dyn. config, both for 1.2 and 1.3 *) ->
+          // cfg: config -> 
 
           // states of the HS components, subject to joint invariant
           epochs: epochs region nonce ->
           nego: Nego.state region r ->
-          log: HandshakeLog.log region -> 
+          log: HandshakeLog.log region (* embedding msg buffers *) -> 
           ks: KeySchedule.ks region r -> 
-          state: rref region role_state -> // state machine; should be opaque
+          state: rref region machineState -> // state machine; should be opaque
           hs
 
 (* the handshake internally maintains epoch
@@ -430,22 +246,8 @@ let i (HS #r0 _ _ _ _ epochs _) rw =
   | Reader -> Epochs.get_reader epochs
   | Writer -> Epochs.get_writer epochs
 
-val handshake_state_init: (cfg:TLSInfo.config) -> (r:role) -> (reg:rid) -> ST (handshake_state r)
-  (requires (fun h -> True))
-  (ensures (fun h0 i h1 -> True))
-let handshake_state_init cfg (r:role) (reg:rid) =
-   let log = HandshakeLog.create #reg in
-   let ks, nonce = KeySchedule.create #reg r log in
-   {hs_nego = None;
-    hs_log = log;
-    hs_ks  = ks;
-    hs_reader = -1;
-    hs_writer = -1;
-    hs_buffers = hs_msg_bufs_init();
-    hs_state =
-        (match r with
-        | Client -> C (C_Idle None)
-        | Server -> S (S_Idle None)) }
+
+
 
 // payload of a handshake fragment, to be made opaque eventually
 type message (i:id) = ( rg: frange i & rbytes rg )
@@ -476,43 +278,6 @@ type incoming =
 
 let in_next_keys (r:incoming) = InAck? r && InAck?.next_keys r
 let in_complete (r:incoming)  = InAck? r && InAck?.complete r
-
-
-(* Handshake API: INTERNAL Callbacks, hidden from API *)
-
-val client_send_client_hello: hs -> ST unit
-  (requires (fun h -> True))
-  (ensures (fun h0 i h1 -> True))
-let client_send_client_hello (HS #r0 r res cfg id lgref hsref) =
-  match (!hsref).hs_state with
-  | C(C_Idle ri) ->
-    let (ClientHello ch,chb) = prepareClientHello cfg ri None (!hsref).hs_ks (!hsref).hs_log  in
-    hsref := {!hsref with
-            hs_buffers = {(!hsref).hs_buffers with hs_outgoing = chb};
-        hs_state = C(C_HelloSent ri ch)}
-
-
-val client_handle_server_hello: hs -> list (hs_msg * bytes) -> ST incoming
-  (requires (fun h -> True))
-  (ensures (fun h0 i h1 -> True))
-let client_handle_server_hello (HS #r0 r res cfg nonce lgref hsref) msgs =
-  match (!hsref).hs_state, msgs with
-  | C(C_HelloSent ri ch),[(ServerHello(sh),l)] ->
-   (match (processServerHello cfg (!hsref).hs_ks (!hsref).hs_log ri ch (ServerHello sh,l)) with
-    | Error z -> InError z
-    | Correct (n,keys) ->
-      // If a handshake encryption key is returned install the epoch and increment the reader
-      (match keys with
-      | Some keys ->
-        let h = Negotiation.Fresh ({session_nego = n}) in
-        let ep = Epochs.recordInstanceToEpoch #r0 #nonce h keys in
-        Epochs.add_epoch lgref ep;
-        Epochs.incr_reader lgref
-      | None -> ());
-      hsref := {!hsref with
-           hs_nego = Some n;
-           hs_state = C(C_HelloReceived n)};
-      InAck (Some? keys) false)
 
 
 let optHashAlg_prime_is_optHashAlg: result hashAlg' -> Tot (result hashAlg) =
@@ -556,16 +321,140 @@ let sigHashAlg_of_ske signature =
   else None
 
 
+(* Handshake API: INTERNAL Callbacks, hidden from API *)
+
+(* Sketch 
+val Nego.prepareClientOffer: config -> clientOffer
+let Nego.prepareClientOffer cfg =
+  let groups = List.Tot.choose CommonDH.group_of_namedGroup cfg.namedGroups in
+  let cipher_suites = ... in
+  let sigAlgs = ... in
+  let protocol_version = ... in
+  let ext = prepareExtensions protocol_version cipher_suites sigAlgs groups kp in
+*)  
+
+
+
+
+(*** Handshake.Client ***)
+
+(*** send ClientHello ***)
+val client_send_client_hello: hs -> ST unit 
+  (requires (fun h -> 
+    True (* add the precondition that Nego and KS are in proper state *) ))
+  (ensures (fun h0 i h1 -> True))
+  (* TODO: what should we say here? something like:
+    - The Keys Schedule state machine is in the initial state
+    - The Handshake log has exactly one more message: the ClientHello computed from the input configurtion
+    - The result is this ClientHello and its serialization
+  *)
+let client_send_client_hello hs =
+  (* merged in prepare_client_hello *)
+  (* Negotiation computes the list of groups from the configuration;
+     KeySchedule computes and serializes the shares from these groups (calling into CommonDH)
+     Messages should do the serialization (calling into CommonDH), but dependencies are tricky
+  *)
+  let offer = Nego.clientOffer hs.nego hs.cfg hs.resume in   (* compute offer from configuration *)
+  let shares = (* compute shares for groups in offer *)
+    match offer.co_protocol_version with
+    | TLS_1p3 -> Some (KeySchedule.ks_client_13_1rtt_init hs.ks offer.co_namedGroups)
+    | _       -> let si = KeySchedule.ks_client_12_init ks in None
+    in
+  (* Some? sido in case of resumption *)
+  let sid =
+    match fst hs.resume with
+    | None -> empty_bytes
+    | Some x -> x
+  in
+  (* In TLSExtensions: prepare client extensions, including key shares *)
+  let ext = prepareExtensions offer hs.resume ri shares in
+  let ch = // a bit too concrete? ClientHello hs.nonce offer hs.resume ri shares
+  {
+    ch_protocol_version = offer.co_protocol_version;
+    ch_client_random = hs.nonce;
+    ch_sessionID = sid;
+    ch_cipher_suites = offer.co_cipher_suites;
+    ch_raw_cipher_suites = None;
+    ch_compressions = offer.co_compressions;
+    ch_extensions = Some ext
+  } in
+  HandshakeLog.send hs.log (ClientHello ch);  // TODO in two steps, appending the binders
+  hs.state := C_HelloSent ri ch
+
+
+(*** receive ServerHello ***)
+let client_ServerHello hs sh =
+    IO.hs_debug_print_string "Processing client hello...\n";
+    let r = Nego.clientModel hs.nego  (*... don't repeat the offer? *) 
+      //ch.ch_extensions ch.ch_protocol_version 
+      sh.sh_protocol_version 
+      sh.sh_server_random 
+      sh.sh_cipher_suite 
+      sh.sh_extensions 
+      sh.sh_compression ri in
+    match r with
+    | Error z -> Error z
+    | Correct (n,keys) -> (
+
+    //17-03-24 what's the main "mode" type? o_nego or mode? 
+   (* no need for this one yet? 
+   let o_nego =
+    {n_client_random = ch.ch_client_random;
+     n_server_random = sh.sh_server_random;
+     n_sessionID = sh.sh_sessionID;
+     n_protocol_version = mode.cm_protocol_version;
+     n_kexAlg = mode.cm_kexAlg;
+     n_aeAlg = mode.cm_aeAlg;
+     n_sigAlg = mode.cm_sigAlg;
+     n_cipher_suite = mode.cm_cipher_suite;
+     n_dh_group = mode.cm_dh_group;
+     n_compression = sh.sh_compression;
+     n_scsv = [];
+     n_extensions = mode.cm_ext;
+     n_resume = false } in 
+     
+    (match o_nego.n_protocol_version, o_nego.n_kexAlg, mode.cm_dh_group, mode.cm_dh_share with
+     | TLS_1p3, Kex_DHE, Some gn, Some gyb
+     | TLS_1p3, Kex_ECDHE, Some gn, Some gyb ->
+       (match CommonDH.group_of_namedGroup gn with
+       | None -> Error(AD_internal_error, perror __SOURCE_FILE__ __LINE__ "Unsupported group negotiated")
+       | Some g ->
+         (match CommonDH.parse g gyb  // This should have been parsed earlier! 
+         with
+         | None -> Error(AD_decode_error, perror __SOURCE_FILE__ __LINE__ "Failed to parse server share")
+         | Some gy ->
+           let keys = KeySchedule.ks_client_13_sh ks o_nego.n_cipher_suite g gy false in
+           Correct (o_nego, Some keys)))
+     | _ -> Correct (o_nego,None))
+*)
+    // split between 1.2 and 1.3 
+      match keys with
+      | Some keys -> // If a handshake encryption key is returned install the epoch and increment the reader
+          let ep = (
+            //? we don't have a full index yet for the epoch; reuse the one for keys??
+            let h = Negotiation.Fresh ({session_nego = n}) in
+            Epochs.recordInstanceToEpoch #r0 #nonce h keys in 
+          Epochs.add_epoch hs.epochs ep;
+          Epochs.incr_reader hs.epochs  )
+      | None -> ());
+      hs_state := C_HelloReceived n;
+      InAck (Some? keys) false )
+
+
+(*** receive Certificate...ServerHelloDone ***)
 // with or without a certificate request; not for TLS 1.3
 val client_ServerHelloDone: 
   hs -> _ -> _ -> _ -> ST incoming
   (requires (fun h -> True))
   (ensures (fun h0 i h1 -> True))
 let client_ServerHelloDone hs c ske ocr = 
-    // nego stuff? 
+    match Nego.clientComplete hs.nego c ske ocr with 
+    | Error z -> Error z 
+    | Correct (fullmode, g, gy) -> (
+
+    (* here are the checks we were doing before; now hopefully in Nego:
     let valid_chain = hs.cfg.check_peer_certificate => Cert.validate_chain c.crt_chain true cfg.peer_name cfg.ca_file in
-    if not valid_chain then Error (AD_certificate_unknown_fatal, perror __SOURCE_FILE__ __LINE__ "Certificate validation failure") 
-    else
+    if not valid_chain then Error (AD_certificate_unknown_fatal, perror __SOURCE_FILE__ __LINE__ "Certificate validation failure")    else
       let ske_tbs = kex_s_to_bytes ske.ske_kex_s in
       let Some cs_sigalg = n.n_sigAlg in
       let sigalgs = n.n_extensions.ne_signature_algorithms in 
@@ -587,29 +476,34 @@ let client_ServerHelloDone hs c ske ocr =
               | None -> Error (AD_handshake_failure, perror __SOURCE_FILE__ __LINE__ "failed to get public key from chain") )
               | Some pk ->
                    let valid_signature = Signature.verify #a h pk tbs sigv in
-                   // IO.print_string("tbs = " ^ (Platform.Bytes.print_bytes tbs) ^ "\n");
-                   IO.print_string("Signature validation status = " ^ (if valid then "OK" else "FAIL") ^ "\n");
+                   // IO.hs_debug_print_string("tbs = " ^ (Platform.Bytes.print_bytes tbs) ^ "\n");
+                   IO.hs_debug_print_string("Signature validation status = " ^ (if valid then "OK" else "FAIL") ^ "\n");
                    if not valid_signature then Error (AD_handshake_failure, perror __SOURCE_FILE__ __LINE__ "failed to check SKE signature")
+                   else 
                      match ske.ske_kex_s with
                      | KEX_S_RSA _ -> Error (AD_handshake_failure, perror __SOURCE_FILE__ __LINE__ "only support ECDHE/DHE SKE") )
-                     | KEX_S_DHE (| g, gy |) -> (
+                     | KEX_S_DHE (| g, gy |) -> 
+                     *)
+
                        ( match ocr with 
                          | None -> ()
                          | Some cr -> 
-                           let cc = {crt_chain = []} in // TODO
-                           HandshakeLog.send (Certificate cc));
+                             let cc = {crt_chain = []} in // TODO
+                             HandshakeLog.send (Certificate cc));
                        let gx = KeySchedule.ks_client_12_full_dh ks n.n_server_random n.n_protocol_version n.n_cipher_suite n.n_extensions.ne_extended_ms g gy in
-                       let cke = {cke_kex_c = kex_c_of_dh_key #g gx} in
-                       let digestClientKeyExchange = HandshakeLog.send_digest (ClientKeyExchange cke) in
+                       let msg = ClientKeyExchange {cke_kex_c = kex_c_of_dh_key #g gx} in
+                       let digestClientKeyExchange = HandshakeLog.send_digest msg  in
 
                        (* fuse these two calls? *)
                        if ems then KeySchedule.ks_client__12_set_session_hash hs.ks digestClientKeyExchange; 
-                       let keys = KeySchedule.ks_12_get_keys (!hsref).hs_ks in
-                       let h = Negotiation.Fresh ({session_nego = n}) in
-                       let ep = Epochs.recordInstanceToEpoch h keys in
-                       Epochs.add_epoch lgref ep;
+                       let app_keys = KeySchedule.ks_12_get_keys hs.ks  in
+                       let ep = 
+                         let h = Negotiation.Fresh ({session_nego = n}) in
+                         Epochs.recordInstanceToEpoch h keys in
+                       Epochs.add_epoch hs.epochs ep;
                        hs.state := C_OutCCS n;                       
                        InAck false false )
+
 
 (*
 val client_send_client_finished: hs -> ST unit
@@ -638,43 +532,33 @@ let client_handle_server_ccs (HS #r0 r res cfg id lgref hsref) msgs =
       InAck true false
     end
 
+(* unused:
+//val client_handle_server_finished: hs -> list (hs_msg * bytes) -> ST incoming
+//  (requires (fun h -> True))
+//  (ensures (fun h0 i h1 -> True))
+let client_handle_server_finished hs f svd (*?*) =
+    let svd = KeySchedule.ks_client_12_server_finished ks in
+    if not (equalBytes svd f.fin_vd) then Error (AD_decode_error, "Finished MAC did not verify")
+    hs.state := C_PostHS;
+    InAck false true
+*)
 
-val processServerFinished: KeySchedule.ks -> HandshakeLog.log -> (hs_msg * bytes) -> ST (result bytes)
-  (requires (fun h -> True))
-  (ensures (fun h0 i h1 -> True))
-let processServerFinished ks log (m,l) =
-   match m with
-   | Finished(f) ->
-     let svd = KeySchedule.ks_client_12_server_finished ks in
-     if (equalBytes svd f.fin_vd) then
-         let _ = log @@ (Finished(f)) in
-    Correct svd
-     else Error (AD_decode_error, "Finished MAC did not verify")
-   | _ -> Error (AD_decode_error, "Unexpected state")
 
-val client_handle_server_finished: hs -> list (hs_msg * bytes) -> ST incoming
-  (requires (fun h -> True))
-  (ensures (fun h0 i h1 -> True))
-let client_handle_server_finished (HS #r0 r res cfg id lgref hsref) msgs =
-  match (!hsref).hs_state, msgs with
-  | C(C_CCSReceived n vd), [(Finished(f),l)] ->
-   (match processServerFinished (!hsref).hs_ks (!hsref).hs_log (Finished f,l) with
-    | Error z -> InError z
-    | Correct svd ->
-       hsref := {!hsref with
-           hs_state = C(C_PostHS)}; // ADL: TODO need a proper renego state Idle (Some (vd,svd)))};
-       InAck false true)
+(*** receive EncryptedExtension...ServerFinished  ***)
+// keep this function check against client ServerHelloDone
+let client_ServerFinished_13 hs ee ocr c cv svd digestCert digestCertVerify digestServerFinished =
+    match Nego.clientComplete_13 hs.nego ee ocr c cv digestCert with 
+    | Error z -> Error z 
+    | Correct full_mode -> 
 
-// TODO check against client ServerHelloDone
-let client_ServerFinished_13 hs ee ocr c cv f =
+    (* here are the checks we were doing before; now hopefully in Nego:
     let valid_chain = cfg.check_peer_certificate => Cert.validate_chain c.crt_chain true cfg.peer_name cfg.ca_file in
     if not valid_chain then Error (AD_decode_error, "Certificate was not valid")
     else
-       let _ = log @@ Certificate(c) in
+    begin
        let Some cs_sigalg = n.n_sigAlg in
        let Some algs = n.n_extensions.ne_signature_algorithms in
-       //let _ = IO.debug_print_string("cv_sig = " ^ (Platform.Bytes.print_bytes cv.cv_sig) ^ "\n") in
-       begin
+       IO.hs_debug_print_string("cv_sig = " ^ (Platform.Bytes.print_bytes cv.cv_sig) ^ "\n");
        match sigHashAlg_of_ske cv.cv_sig with
        | Some ((sa,ha), sigv) ->
          if not (List.Tot.existsb (fun (xs,xh) -> (xs = sa && xh = ha)) (list_sigHashAlg_is_list_tuple_sig_hash algs))
@@ -692,33 +576,103 @@ let client_ServerFinished_13 hs ee ocr c cv f =
            | None -> Error (AD_decode_error, "Certificate was not valid")
            | Some pk ->
              let valid_signature = Signature.verify ha pk tbs sigv in
-             IO.print_string("Signature validation status = " ^ (if valid then "OK" else "FAIL") ^ "\n");
+             IO.hs_debug_print_string("Signature validation status = " ^ (if valid then "OK" else "FAIL") ^ "\n");
              if not valid then Error (AD_decode_error, "Certificate signature did not verify")
-             else
-               let _ = log @@ CertificateVerify(cv) in
-               let svd = KeySchedule.ks_client_13_server_finished ks in
-               if  not (equalBytes svd f.fin_vd) then Error (AD_decode_error, "Finished MAC did not verify")
-               else
-                 let _ = log @@ (Finished(f)) in
-                 let keys = KeySchedule.ks_client_13_sf ks in
-                 let cvd = KeySchedule.ks_client_13_client_finished ks in
-                 let cfin = {fin_vd = cvd} in
-                 ( match ocr with 
-                   | Some cr -> HandshakeLog.send (Certificate {crt_chain = []})
-                   | None -> () )
-                 HandshakeLog.send (Finished cfin);
-                 let ems = KeySchedule.ks_client_13_cf ks in
+             else *)
 
-                 let h = Negotiation.Fresh ({session_nego = n}) in
-                 let ep = Epochs.recordInstanceToEpoch #r0 #id h keys in
-                 Epochs.add_epoch lgref ep;
-                 Epochs.incr_reader lgref;
-                 Epochs.incr_writer lgref; // TODO update writer key properly
-                 let (fb, cvd) = (match hsl with
-                 hs.state := C_FinishedReceived n (cvd,svd);
-                 InAck true false )
+               let (cfin_key, sfin_key, app_keys) = KeySchedule.ks_client_13_server_finished ks in
+               // was also calling:  let keys = KeySchedule.ks_client_13_sf ks in
+               // was also calling:  let cvd = KeySchedule.ks_client_13_client_finished ks in
+               // was also calling: let ems = KeySchedule.ks_client_13_cf ks in // ? 
+               if  not MAC.verify sfin_key digestCertVerify svd then Error (AD_decode_error, "Finished MAC did not verify")
+               else (
+                 let digest = 
+                   match ocr with 
+                   | Some cr -> HandshakeLog.send_digest (Certificate {crt_chain = []}) 
+                   | None -> digestServerFinished in 
+                 let cvd = MAC.mac cfin_key digest in 
+                 Handshake.Log.send (Finished {fin_vd = cvd};
+                 let ep = 
+                   let h = Negotiation.Fresh ({session_nego = full_mode}) in // review index?
+                   Epochs.recordInstanceToEpoch #r0 #id h app_keys in
+                 Epochs.add_epoch hs.epochs ep;
+                 Epochs.incr_reader hs.epochs;
+                 Epochs.incr_writer hs.epochs; // TODO update writer key properly
+                 hs.state := C_FinishedReceived full_mode (cvd,svd); // do we still need to keep those?
+                 InAck true false ))
 
 
+
+(*** Handshake.Server ***)
+
+(*** send ServerHello ***) 
+// FIXME: TLS1.3
+// no point sharing between TLS 1.2 and TLS 1.3?
+val prepareServerHello: 
+  st: hs {st.role = Server} -> 
+  // config -> 
+  // KeySchedule.ks -> 
+  // HandshakeLog.log -> 
+  // option ri -> 
+  // (hs_msg * bytes) -> 
+  ST (result (nego * option KeySchedule.recordInstance * (hs_msg * bytes)))
+  (requires (fun h -> True))
+  (ensures (fun h0 i h1 -> True))
+let prepareServerHello hs (* cfg ks log ri (ClientHello ch,_) *) =
+ let negotiated = Nego.computeServerMode hs.nego hs.cfg  (* ch.ch_protocol_version ch.ch_cipher_suites ch.ch_extensions ch.ch_compressions *) hs.resume in
+  match negotiated with
+   | Error z -> Error z
+   | Correct mode ->
+     let srand = KS.ks_server_random ks in
+     let ksl =
+       (match mode.sm_protocol_version, mode.sm_dh_group, mode.sm_dh_share with
+       | TLS_1p3, Some gn, Some gxb ->
+         (match CommonDH.group_of_namedGroup gn with
+         | None -> None
+         | Some g ->
+           (match CommonDH.parse g gxb with
+           | None -> None
+           | Some gx ->
+             Some (KeySchedule.ks_server_13_1rtt_init ks ch.ch_client_random mode.sm_cipher_suite g gx)))
+       | _ -> None) in
+    (* TLSExtensions:negotiateServerExtensions *)
+    match negotiateServerExtensions mode.sm_protocol_version ch.ch_extensions ch.ch_cipher_suites cfg mode.sm_cipher_suite ri ksl false with
+    | Error(z) -> Error(z)
+    | Correct(sext) ->
+      let sid = CoreCrypto.random 32 in
+      let sh =
+      {sh_protocol_version = mode.sm_protocol_version;
+       sh_sessionID = Some sid;
+       sh_server_random = srand;
+       sh_cipher_suite = mode.sm_cipher_suite;
+       sh_compression = mode.sm_comp;
+       sh_extensions = sext} in
+      let nego =
+      {n_client_random = ch.ch_client_random;
+       n_server_random = srand;
+       n_sessionID = Some sid;
+       n_protocol_version = mode.sm_protocol_version;
+       n_kexAlg = mode.sm_kexAlg;
+       n_sigAlg = mode.sm_sigAlg;
+       n_aeAlg  = mode.sm_aeAlg;
+       n_cipher_suite = mode.sm_cipher_suite;
+       n_compression = mode.sm_comp;
+       n_dh_group = mode.sm_dh_group;
+       n_scsv = [];
+       n_extensions = mode.sm_ext;
+       (* [getCachedSession] returned [None], so no session resumption *)
+       n_resume = false} in
+       let _ = log @@ (ClientHello ch) in
+       let shb = log @@ (ServerHello sh) in
+       let keys = (match mode.sm_protocol_version with
+               | TLS_1p3 ->
+             let keys = KeySchedule.ks_server_13_sh ks in
+             Some keys
+           | _ -> None) in
+             Correct (nego,keys,(ServerHello sh,shb))
+
+
+(*** receive ServerHello ***) 
 val server_handle_client_hello: hs -> list (hs_msg * bytes) -> ST incoming
   (requires (fun h -> True))
   (ensures (fun h0 i h1 -> True))
@@ -745,14 +699,19 @@ let server_handle_client_hello (HS #r0 r res cfg id lgref hsref) msgs =
        InAck false false)
 
 
-let prepareServerHelloDone cfg n ks log =
-    if (n.n_protocol_version <> TLS_1p3 && Some? n.n_sigAlg &&
-       (n.n_kexAlg = Kex_DHE || n.n_kexAlg = Kex_ECDHE))
-    then
+(*** send ServerHelloDone ***) 
+
+//val server_ServerHelloDone: hs -> ST unit
+//  (requires (fun h -> True))
+//  (ensures (fun h0 i h1 -> True))
+let server_ServerHelloDone hs n =
+    if not (n.n_protocol_version <> TLS_1p3 && Some? n.n_sigAlg && (n.n_kexAlg = Kex_DHE || n.n_kexAlg = Kex_ECDHE))
+    then Error (AD_handshake_failure, perror __SOURCE_FILE__ __LINE__ "should not call this function in TLS 1.3")
+    else 
     match Cert.lookup_chain cfg.cert_chain_file with
+    | Error z -> Error z
     | Correct chain ->
       let c = {crt_chain = chain} in
-      let cb = log @@ Certificate(c) in
       let cr = n.n_client_random in
       let ems = n.n_extensions.ne_extended_ms in
       let pv = n.n_protocol_version in
@@ -760,7 +719,6 @@ let prepareServerHelloDone cfg n ks log =
       let Some gn = n.n_dh_group in // FIXME error flow
       let Some g = CommonDH.group_of_namedGroup gn in // FIXME static enforcement
       let gy = KeySchedule.ks_server_12_init_dh ks cr pv cs ems g in
-
       let kex_s = KEX_S_DHE gy in
       let sv = kex_s_to_bytes kex_s in
       let csr = n.n_client_random @| n.n_server_random in
@@ -771,8 +729,7 @@ let prepareServerHelloDone cfg n ks log =
       let algs =
           match sigalgs with
           | Some l -> l
-          | None -> [(sa,Hash Hashing.Spec.SHA1)]
-        in
+          | None -> [(sa,Hash Hashing.Spec.SHA1)]  in
       let algs = List.Tot.filter (fun (s,_) -> s = sa) algs in
       let sa, ha =
           match algs with
@@ -784,140 +741,88 @@ let prepareServerHelloDone cfg n ks log =
       let tbs = to_be_signed n.n_protocol_version Server (Some csr) sv in
       begin
         match Signature.lookup_key #a cfg.private_key_file with
+        | None -> Error (AD_internal_error, perror __SOURCE_FILE__ __LINE__ "could not load siginig key")
         | Some csk ->
             let sigv = Signature.sign ha csk tbs in
-          if length sigv >= 2 && length sigv < 65536 then
+          if not (length sigv >= 2 && length sigv < 65536)
+          then Error (AD_decode_error, perror __SOURCE_FILE__ __LINE__ "signature length out of range")
+          else
+
+      // move most code above to Nego?   
               begin
-              lemma_repr_bytes_values (length sigv);
-              let signature = (hab @| sab @| (vlbytes 2 sigv)) in
-              let ske = {ske_kex_s = kex_s; ske_sig = signature} in
-                  let skeb = log @@ ServerKeyExchange(ske) in
-                  let shdb = log @@ ServerHelloDone in
-              Correct [(Certificate(c),cb);(ServerKeyExchange(ske),skeb);(ServerHelloDone,shdb)]
+                lemma_repr_bytes_values (length sigv);
+                let signature = (hab @| sab @| (vlbytes 2 sigv)) in
+                let ske = {ske_kex_s = kex_s; ske_sig = signature} in
+                Handshake.Log.send (Certificate c);
+                Handshake.Log.send (ServerKeyExchange ske);
+                Handshake.Log.send ServerHelloDone;
+                s.state := S_HelloDone n
               end
-            else
-            Error (AD_decode_error, perror __SOURCE_FILE__ __LINE__ "signature length out of range")
-        | None -> Error (AD_internal_error, perror __SOURCE_FILE__ __LINE__ "could not load siginig key")
       end
-    | Error z -> Error z
-  else
-    Error (AD_handshake_failure, perror __SOURCE_FILE__ __LINE__ "should not call this function in TLS 1.3")
 
-val server_send_server_hello_done: hs -> ST unit
-  (requires (fun h -> True))
-  (ensures (fun h0 i h1 -> True))
-let server_send_server_hello_done (HS #r0 r res cfg id lgref hsref) =
-  match (!hsref).hs_state with
-  | S(S_HelloSent n)
-    when (n.n_protocol_version <> TLS_1p3 &&
-     (n.n_kexAlg = Kex_DHE || n.n_kexAlg = Kex_ECDHE)) ->
-    (match prepareServerHelloDone cfg n (!hsref).hs_ks (!hsref).hs_log with
-     | Correct ([(Certificate(c),cb);(ServerKeyExchange(ske),skeb);(ServerHelloDone,shdb)]) ->
-         let nl = cb @| skeb @| shdb in
-        hsref := {!hsref with
-         hs_buffers = {(!hsref).hs_buffers with hs_outgoing = nl};
-         hs_state = S(S_HelloDone n)}
-      | Error e ->
-      hsref := {!hsref with hs_state = S(S_Error e)})
+(*** receive Client CCS ***)
+let server_ClientCCS hs cke digest (* clientCert *)  =
+    // FIXME support optional client c and cv 
+    // let ems = n.n_extensions.ne_extended_ms in // ask Nego? 
+    match cke.cke_kex_c with
+      | KEX_C_RSA _ | KEX_C_DH -> Error(AD_decode_error, perror __SOURCE_FILE__ __LINE__ "Expected DHE/ECDHE CKE")
+      | KEX_C_DHE gyb
+      | KEX_C_ECDHE gyb -> (
+          let Some gn = n.n_dh_group in // FIXME error flow
+          let Some g = CommonDH.group_of_namedGroup gn in // FIXME static enforcement
+          let gy = CommonDH.parse g gyb in 
+          KeySchedule.ks_server_12_cke_dh ks g gy; 
 
-let processClientCCS n ks log msgs opt_msgs =
-    let rem =
-    match opt_msgs with
-    | [(Certificate c,_)] ->
-      let _ = log @@ Certificate(c) in
-      Correct msgs
-    | [] -> Correct msgs
-    | _ -> Error(AD_decode_error, perror __SOURCE_FILE__ __LINE__ "Expected Certificate only before CKE") in
-    match rem with
-    | Correct [(ClientKeyExchange cke,_)] ->
-      let ems = n.n_extensions.ne_extended_ms in
-      let _ = log @@ ClientKeyExchange(cke) in
-      (match cke.cke_kex_c with
-       | KEX_C_DHE gyb
-       | KEX_C_ECDHE gyb ->
-         let Some gn = n.n_dh_group in // FIXME error flow
-         let Some g = CommonDH.group_of_namedGroup gn in // FIXME static enforcement
-         let gy = CommonDH.parse g gyb in
-         KeySchedule.ks_server_12_cke_dh ks g gy;
-           Correct ()
-       | _ -> Error(AD_decode_error, perror __SOURCE_FILE__ __LINE__ "Expected DHE/ECDHE CKE"))
-    | Error z -> Error z
-
-val server_handle_client_ccs: hs -> list (hs_msg * bytes) -> list (hs_msg * bytes) -> ST incoming
-  (requires (fun h -> True))
-  (ensures (fun h0 i h1 -> True))
-
-let server_handle_client_ccs (HS #r0 r res cfg id lgref hsref) msgs opt_msgs =
-  match (!hsref).hs_state with
-  | S(S_HelloDone n) when
-     (n.n_protocol_version <> TLS_1p3 &&
-      (n.n_kexAlg = Kex_DHE || n.n_kexAlg = Kex_ECDHE)) ->
-     (match processClientCCS n (!hsref).hs_ks (!hsref).hs_log msgs opt_msgs with
-      | Correct () ->
-        let keys = KeySchedule.ks_12_get_keys (!hsref).hs_ks in
-        let h = Negotiation.Fresh ({session_nego = n}) in
-        let ep = Epochs.recordInstanceToEpoch h keys in
-        Epochs.add_epoch lgref ep;
-        Epochs.incr_reader lgref;
-        (hsref := {!hsref with
-           hs_state = S(S_CCSReceived n)};
-         InAck true false)
-      | Error z -> InError z)
+          let app_keys = KeySchedule.ks_12_get_keys (!hsref).hs_ks in
+          let h = Negotiation.Fresh ({session_nego = n}) in
+          let ep = Epochs.recordInstanceToEpoch h keys in
+          Epochs.add_epoch lgref ep;
+          Epochs.incr_reader lgref;
+          hs.state := S_CCSReceived n digest;
+          InAck true false )
 
 
-let processClientFinished n ks log msgs =
-    match msgs with
-    | [(Finished f,_)] ->
-      let cvd = KeySchedule.ks_server_12_client_finished ks in
-      if (equalBytes cvd f.fin_vd) then
-        let _ = log @@ Finished(f) in
+(*** Receive ClientFinish ***) 
+let server_ClientFinished hs digestCCS digestClientFinished =
+
+    // to be adjusted
+    let cvd = KeySchedule.ks_server_12_client_finished ks in
+    if not (equalBytes cvd f.fin_vd) then Error (AD_decode_error, "Finished MAC did not verify")
+    else
         let svd = KeySchedule.ks_server_12_server_finished ks in
         let fin = Finished ({fin_vd = svd}) in
         let finb = log @@ fin in
-        Correct [(fin,finb)]
-      else Error (AD_decode_error, "Finished MAC did not verify")
-   | _ -> Error (AD_unexpected_message, perror __SOURCE_FILE__ __LINE__ "ClientFinished expected")
 
-val server_handle_client_finished: hs -> list (hs_msg * bytes) -> ST incoming
-  (requires (fun h -> True))
-  (ensures (fun h0 i h1 -> True))
-
-let server_handle_client_finished (HS #r0 r res cfg id lgref hsref) msgs =
-  match (!hsref).hs_state with
-  | S(S_CCSReceived n) ->
-    match processClientFinished n (!hsref).hs_ks (!hsref).hs_log msgs with
-    | Correct [(Finished(f),finb)] ->
         (hsref := {!hsref with
                   hs_buffers = {(!hsref).hs_buffers with
-                   hs_outgoing_ccs = true; // Because of the current constraints of the Record/HS interface the sendCCS flag is only available on writing
+                   hs_outgoing_ccs = true; 
+                   // Because of the current constraints of the Record/HS interface the sendCCS flag is only available on writing
                    // therefore, I am forced to "buffer" the fact a CCS will need to be sent before the ServerFinished
                    hs_outgoing = finb};
                hs_state = S(S_OutCCS n)};
-         InAck false false)
-    | Error e -> InError e
+        InAck false false)
 
-val server_send_server_finished: hs -> ST unit
-  (requires (fun h -> True))
-  (ensures (fun h0 i h1 -> True))
-let server_send_server_finished (HS #r0 r res cfg id lgref hsref) =
+let server_send_server_finished hs n =
   match (!hsref).hs_state with
   | S(S_OutCCS n) ->
     hsref := {!hsref with
            hs_state = S(S_FinishedSent n)}
 
 
+(*** Send ServerFinish ***)
+val server_send_server_finished_13: hs -> ST unit
+  (requires (fun h -> True))
+  (ensures (fun h0 i h1 -> True))
+let server_send_server_finished_13 hs n = 
 
-
-let prepareServerFinished_13 cfg n ks log =
-    if (n.n_protocol_version = TLS_1p3 && Some? n.n_sigAlg &&
-       (n.n_kexAlg = Kex_DHE || n.n_kexAlg = Kex_ECDHE))
-    then
-    let ee = {ee_extensions = []} in
-    let eeb = log @@ EncryptedExtensions(ee) in
+    if not (n.n_protocol_version = TLS_1p3 && Some? n.n_sigAlg && (n.n_kexAlg = Kex_DHE || n.n_kexAlg = Kex_ECDHE))
+    then Error (AD_handshake_failure, perror __SOURCE_FILE__ __LINE__ "should not call this function in TLS < 1.3")
+    else 
+    Handshake.Log.send (EncryptedExtensions {ee_extensions = []});
     match Cert.lookup_chain cfg.cert_chain_file with
+    | Error z -> Error z
     | Correct chain ->
-      let c = {crt_chain = chain} in
-      let cb = log @@ Certificate(c) in
+      Handshake.Log.send (Certificate {crt_chain = chain});
       let pv = n.n_protocol_version in
       let cs = n.n_cipher_suite in
       let sh_alg = sessionHashAlg pv cs in
@@ -926,106 +831,61 @@ let prepareServerFinished_13 cfg n ks log =
       // If no signature nego took place we use the SA and KDF hash from the CS
       let Some sa = n.n_sigAlg in
       let algs =
-    match n.n_extensions.ne_signature_algorithms with
+        match n.n_extensions.ne_signature_algorithms with
         | Some l -> l
         | None -> [sa, sh_alg]
       in
       let algs = List.Tot.filter (fun (s,_) -> s = sa) algs in
       let sa, ha =
-    match algs with
-    | ha::_ -> ha
-    | [] -> (sa, sh_alg) in
+        match algs with
+        | ha::_ -> ha
+        | [] -> (sa, sh_alg) in
       let hab, sab = hashAlgBytes ha, sigAlgBytes sa in
       let a = Signature.Use (fun _ -> true) sa [ha] false false in
       begin
-      match Signature.lookup_key #a cfg.private_key_file with
-      | Some csk ->
-        let Hash sh_alg = sh_alg in
-        let hL = hashSize sh_alg in
-        let zeroes = Platform.Bytes.abytes (String.make hL (Char.char_of_int 0)) in
-        let rc = Hashing.compute  sh_alg zeroes in
-        let lb = (HandshakeLog.getHash log sh_alg) @| rc in
-        let tbs = to_be_signed pv Server None lb in
-        let sigv = Signature.sign ha csk tbs in
-    let signature = (hab @| sab @| (vlbytes 2 sigv)) in
-        let scv = {cv_sig = signature} in
-        let scvb = log @@ CertificateVerify(scv) in
-    let svd = KeySchedule.ks_server_13_server_finished ks in
-    let fin = {fin_vd = svd} in
-    let finb = log @@ Finished(fin) in
-        let keys = KeySchedule.ks_server_13_sf ks in
-    Correct ([(EncryptedExtensions(ee),eeb);(Certificate(c),cb);(CertificateVerify(scv),scvb);(Finished(fin),finb)], keys)
-      | None -> Error (AD_internal_error, perror __SOURCE_FILE__ __LINE__ "could not load signing key")
-      end
-    | Error z -> Error z
-    else
-       Error (AD_handshake_failure, perror __SOURCE_FILE__ __LINE__ "should not call this function in TLS < 1.3")
-
-val server_send_server_finished_13: hs -> ST unit
-  (requires (fun h -> True))
-  (ensures (fun h0 i h1 -> True))
-let server_send_server_finished_13 (HS #r0 r res cfg id lgref hsref) =
-  match (!hsref).hs_state with
-  | S(S_HelloSent n)
-    when (n.n_protocol_version = TLS_1p3 &&
-     (n.n_kexAlg = Kex_DHE || n.n_kexAlg = Kex_ECDHE)) ->
-    (match prepareServerFinished_13 cfg n (!hsref).hs_ks (!hsref).hs_log with
-     | Correct ([(EncryptedExtensions(ee),eeb);(Certificate(c),cb);(CertificateVerify(scv),scvb);(Finished(f),sfinb)], keys) ->
-            let nl = eeb @| cb @| scvb @| sfinb in
-            let h = Negotiation.Fresh ({session_nego = n}) in
-            let ep = Epochs.recordInstanceToEpoch #r0 #id h keys in
+        match Signature.lookup_key #a cfg.private_key_file with
+        | None -> Error (AD_internal_error, perror __SOURCE_FILE__ __LINE__ "could not load signing key")
+        | Some csk ->
+            let Hash sh_alg = sh_alg in
+            let hL = hashSize sh_alg in
+            let zeroes = Platform.Bytes.abytes (String.make hL (Char.char_of_int 0)) in
+            let rc = Hashing.compute  sh_alg zeroes in
+            let lb = (HandshakeLog.getHash log sh_alg) @| rc in
+            let tbs = to_be_signed pv Server None lb in
+            let sigv = Signature.sign ha csk tbs in
+            let signature = (hab @| sab @| (vlbytes 2 sigv)) in
+            Handshake.Log.send (CertificateVerify {cv_sig = signature}) in
+            let svd = KeySchedule.ks_server_13_server_finished ks in
+            Handshake.Log.send (Finished {fin_vd = svd}) in
+            let keys = KeySchedule.ks_server_13_sf ks in
+            let ep = 
+               let h = Negotiation.Fresh ({session_nego = n}) in
+               Epochs.recordInstanceToEpoch #r0 #id h keys in
             Epochs.add_epoch lgref ep;
             Epochs.incr_writer lgref; // Switch to ATK after the SF
             Epochs.incr_reader lgref; // TODO when to increment the reader?
-        hsref := {!hsref with
-         hs_buffers = {(!hsref).hs_buffers with hs_outgoing = nl; hs_outgoing_epochchange = Some Writer; };
-         hs_state = S(S_FinishedSent n)}
-     | Error e ->
-      hsref := {!hsref with hs_state = S(S_Error e)})
+
+            ///??? hs_outgoing_epochchange = Some Writer; };
+            hs.state := S_FinishedSent n
+      end
 
 
-val processClientFinished_13: KeySchedule.ks -> HandshakeLog.log -> list (hs_msg * bytes) -> list (hs_msg * bytes) ->
-                      ST (result (bytes))
-  (requires (fun h -> True))
-  (ensures (fun h0 i h1 -> True))
-let processClientFinished_13 ks log msgs opt_msgs =
-   let rem =
-   match opt_msgs with
-   | [(Certificate c,_); (CertificateVerify cv,_)] ->
-     let _ = log @@ Certificate(c) in
-     let _ = log @@ CertificateVerify(cv) in
-     Error(AD_internal_error, perror __SOURCE_FILE__ __LINE__ "Client CertificateVerify validation not implemented")
-   | [] -> Correct msgs
-   | _ -> Error(AD_decode_error, perror __SOURCE_FILE__ __LINE__ "Expected Cert+CertVerify") in
-   match rem with
-   | Correct ([(Finished(f),finb)]) ->
-     let cvd = KeySchedule.ks_server_13_client_finished ks in
-     if (equalBytes cvd f.fin_vd) then
-         let _ = log @@ (Finished(f)) in
-    Correct cvd
-     else Error (AD_decode_error, "Finished MAC did not verify")
-   | _ -> Error (AD_decode_error, "Unexpected state")
+(*** receive ClientFinish ***)
+let server_ClientFinished_13 hs n f digest clientAuth=
+   match clientAuth with
+   | Some (c,cv) -> Error(AD_internal_error, perror __SOURCE_FILE__ __LINE__ "Client CertificateVerify validation not implemented")
+   | None -> 
+       let cvd = KeySchedule.ks_server_13_client_finished ks in
+       if not (equalBytes cvd f.fin_vd) then Error (AD_decode_error, "Finished MAC did not verify")
+       else (
+          Epochs.incr_writer hs.epochs lgref;
+          hs.state := S_FinishedReceived n;
+          InAck true false )
 
-
-val server_handle_client_finished_13: hs -> list (hs_msg * bytes) -> list (hs_msg * bytes) -> ST incoming
-  (requires (fun h -> True))
-  (ensures (fun h0 i h1 -> True))
-let server_handle_client_finished_13 (HS #r0 r res cfg id lgref hsref) msgs opt_msgs =
-  match (!hsref).hs_state with
-  | S(S_FinishedSent n) ->
-    (match processClientFinished_13 (!hsref).hs_ks (!hsref).hs_log msgs opt_msgs with
-     | Correct cvd ->
-        Epochs.incr_writer lgref;
-        hsref := {!hsref with hs_state = S(S_FinishedReceived n)};
-        InAck true false
-     | Error z -> InError z)
-
-
-(* TODO: resumption *)
+(*** TODO: resumption ***)
 assume val server_send_server_finished_res: hs -> ST unit
   (requires (fun h -> True))
   (ensures (fun h0 i h1 -> True))
-
 
 
 
@@ -1055,7 +915,7 @@ let iT_old (HS r res cfg id l st) rw =
 (*** Control Interface ***)
 
 // Create instance for a fresh connection, with optional resumption for clients
-val init: r0:rid -> r: role -> cfg:config -> resume: resume_id r ->
+val create: r0:rid -> r: role -> cfg:config -> resume: resume_id r ->
   ST hs
   (requires (fun h -> True))
   (ensures (fun h0 s h1 ->
@@ -1066,12 +926,25 @@ val init: r0:rid -> r: role -> cfg:config -> resume: resume_id r ->
     HS?.resume s = resume /\
     HS?.cfg s = cfg /\
     logT s h1 = Seq.createEmpty ))
-let init r0 r cfg res =
+let create r0 r cfg res =
     let id = Nonce.mkHelloRandom r r0 in //NS: should this really be Client?
     let lgref = Epochs.epochs_init r0 id in
     let hs = handshake_state_init cfg r r0 in
     let hsref = ralloc r0 hs in
     HS #r0 r res cfg id lgref hsref
+
+// MERGE: 
+val handshake_state_init: (cfg:TLSInfo.config) -> (r:role) -> (reg:rid) -> ST (handshake_state r)
+  (requires (fun h -> True))
+  (ensures (fun h0 i h1 -> True))
+let handshake_state_init cfg (r:role) (reg:rid) =
+   let nego = Nego.create cfg in // where is the resumption info? 
+   let log = HandshakeLog.create #reg in
+   let ks, nonce = KeySchedule.create #reg r log in
+   let epochs = Epochs.create reg nonce
+   let state = ralloc (if r = Client then C_Idle else S_Idle) in
+   ST r nonce epochs nego log ks state
+
 
 let mods s h0 h1 =
   HyperStack.modifies_one s.region h0 h1
@@ -1140,6 +1013,7 @@ let rec next_fragment i hs =
        | Some n -> Some n.n_protocol_version, Some n.n_kexAlg, Some n.n_resume) in
     let b = (!hsref).hs_buffers.hs_outgoing in
 
+    // GOING to Handshake.Log
     //16-06-01 TODO: handle fragmentation; return fragment + flags set in some cases
     let l = length b in
     if (!hsref).hs_buffers.hs_outgoing_ccs then (
@@ -1154,21 +1028,21 @@ let rec next_fragment i hs =
           | None -> false
           | Some Reader -> Epochs.incr_reader lgref; true // possibly used by server in 0-RT
           | Some Writer -> Epochs.incr_writer lgref; true in
-       let tbb =
-        if hs_debug then
-          IO.debug_print_string (" *** WRITE "^(print_bytes b)^"\n")
-        else false in
+       IO.hs_debug_print_string (" *** WRITE "^print_bytes b^"\n");
        hsref := {!hsref with
          hs_buffers = {(!hsref).hs_buffers with
            hs_outgoing = empty_bytes;
            hs_outgoing_epochchange = None }};
        Outgoing (Some (out_msg i (l,l) b)) false keychange false)
     else
+    
       (match (!hsref).hs_state with
        | C (C_Error e) -> OutError e
        | S (S_Error e) -> OutError e
-       | C (C_Idle ri) -> (client_send_client_hello hs; next_fragment i hs)
-      | C_OutCCS n -> (
+       | C_Idle ri -> (
+          client_send_client_hello hs; 
+          next_fragment i hs )
+       | C_OutCCS n -> (
           //was: client_send_client_finished hs;
           let tag = KeySchedule.ks_client_12_client_finished hs.ks in
           HandshakeLog.send (Finished {fin_vd = tag});
@@ -1180,13 +1054,13 @@ let rec next_fragment i hs =
           Epochs.incr_writer lgref; // Switch to ATK writer
           Outgoing None false true true
        | S (S_HelloSent n) when (Some? pv && pv <> Some TLS_1p3 && res = Some false) ->
-          server_send_server_hello_done hs;
+          server_ServerHelloDone hs n;
           next_fragment i hs
        | S (S_HelloSent n) when (Some? pv && pv <> Some TLS_1p3 && res = Some true) ->
           server_send_server_finished_res hs;
           next_fragment i hs
        | S (S_HelloSent n) when (Some? pv && pv = Some TLS_1p3) ->
-          server_send_server_finished_13 hs;
+          server_send_server_finished_13 hs n;
           next_fragment i hs
        | S (S_FinishedReceived n) ->
           Epochs.incr_reader lgref; // Switch to ATK reader
@@ -1199,12 +1073,13 @@ let rec next_fragment i hs =
 
 (*** Incoming (main) ***)
 
+// GOING Handshake.Log
 val parseHandshakeMessages : option protocolVersion -> option kexAlg -> buf:bytes -> Tot  (result (rem:bytes * list (hs_msg * bytes)))
 let rec parseHandshakeMessages pv kex buf =
     match parseMessage buf with
     | Error z -> Error z
-    | Correct(None) -> Correct (buf,[])
-    | Correct(Some (|rem,hstype,pl,to_log|)) ->
+    | Correct None -> Correct (buf,[])
+    | Correct (Some (|rem,hstype,pl,to_log|)) ->
       (match parseHandshakeMessage pv kex hstype pl with
        | Error z -> Error z
        | Correct hsm ->
@@ -1265,42 +1140,33 @@ let recv_fragment hs #i f =
         else false in
       *)
 
-    match !hsref.hs_state, flight with 
+    (* incoming transitions for our state machine *) 
+    match !hs.state, flight with 
+
+      (* CLIENT *) 
+      
       | C_Idle, _ -> InError(AD_unexpected_message, "Client hasn't sent hello yet")
 
-      | C_HelloSent ch, ([ServerHello sh], [digestServerHello]) -> (
-           IO.print_string "Processing client hello...\n";
-           (* adapted from client_handle_client_hello; handling all TLS version so far *)
-           let pv = sh.sh_protocol_version = TLS_1p3 in 
-           match processServerHello cfg (!hsref).hs_ks (!hsref).hs_log ri ch (ServerHello sh,l) with
-               | Error z -> InError z
-               | Correct (n,keys) -> // If a handshake encryption key is returned install the epoch and increment the reader
-                 match keys with
-                 | Some keys ->
-                   let h = Negotiation.Fresh ({session_nego = n}) in
-                   let ep = Epochs.recordInstanceToEpoch #r0 #nonce h keys in 
-                   ( Epochs.add_epoch lgref ep;
-                     Epochs.incr_reader lgref )
-                 | None -> ();
-              hs_state := C_HelloReceived n;
-              InAck (Some? keys) false )
+      | C_HelloSent ch, ([ServerHello sh], [digestServerHello]) -> client_ServerHello sh digestServerHello
 
       | C_HelloReceived n, ([Certificate c; ServerKeyExchange ske; ServerHelloDone], [])
-        when Some? pv && pv <> Some TLS_1p3 && res = Some false && (kex = Some Kex_DHE || kex = Some Kex_ECDHE) ->
+        when (Some? pv && pv <> Some TLS_1p3 && res = Some false && (kex = Some Kex_DHE || kex = Some Kex_ECDHE)) ->
           (* shall we also check we have a sigAlg? *)
           client_ServerHelloDone hs c ske None
 
       | C_HelloReceived n, ([Certificate c; ServerKeyExchange ske; CertificateRequest cr; ServerHelloDone], [])
-        when Some? pv && pv <> Some TLS_1p3 && res = Some false && (kex = Some Kex_DHE || kex = Some Kex_ECDHE) ->
+        when (Some? pv && pv <> Some TLS_1p3 && res = Some false && (kex = Some Kex_DHE || kex = Some Kex_ECDHE)) ->
           client_ServerHelloDone hs c ske (Some cr)
 
-      | C_HelloReceived n, ([EncryptedExtensions ee; Certificate c; CertificateVerify cv; Finished f], [...]) 
+      | C_HelloReceived n, ([EncryptedExtensions ee; Certificate c; CertificateVerify cv; Finished f], [digestCert; digestCertVerify; digestServerFinished]) 
         when (Some? pv && pv = Some TLS_1p3 && (kex = Some Kex_DHE || kex = Some Kex_ECDHE)) ->
-          client_ServerFinished_13 hs ee None c cv f
+          client_ServerFinished_13 hs ee None c cv f.fin_vd digestCert digestCertVerify digestServerFinished
 
-      | C_HelloReceived n, ([EncryptedExtensions ee; CertificateRequest cr; Certificate c; CertificateVerify cv; Finished f], [...]) 
+      | C_HelloReceived n, ([EncryptedExtensions ee; CertificateRequest cr; Certificate c; CertificateVerify cv; Finished f], [digestCert; digestCertVerify; digestServerFinished]) 
         when (Some? pv && pv = Some TLS_1p3 && (kex = Some Kex_DHE || kex = Some Kex_ECDHE)) ->
-          client_ServerFinished_13 hs ee (Some cr) c cv f
+          client_ServerFinished_13 hs ee (Some cr) c cv f.fin_vd digestCert digestCertVerify digestServerFinished
+
+      // we'll have other variants for resumption, shc as ([EncryptedExtensions ee; Finished f], [...]) 
 
       | C_CCSReceived n cv, ([Finished f], [digestServerFinished]) 
         when Some? pv && pv <> Some TLS_1p3 ->
@@ -1310,31 +1176,29 @@ let recv_fragment hs #i f =
             InAck false true )
           else Error (AD_decode_error, "Finished MAC did not verify")
 
-      | S (S_Idle ri), (ClientHello(ch),l)::hsl ->
-       hsref := {!hsref with hs_buffers = {(!hsref).hs_buffers with hs_incoming_parsed = hsl}};
-               server_handle_client_hello hs
-               [(ClientHello(ch),l)]
-       | S (S_CCSReceived s), (Finished(f),l)::hsl
-         when (Some? pv && pv <> Some TLS_1p3) ->
-       hsref := {!hsref with hs_buffers = {(!hsref).hs_buffers with hs_incoming_parsed = hsl}};
-               server_handle_client_finished hs
-               [(Finished(f),l)]
+      (* SERVER *) 
 
-       | S (S_FinishedSent s), (Finished(f),l')::[]
-         when (Some? pv && pv = Some TLS_1p3) ->
-       hsref := {!hsref with hs_buffers = {(!hsref).hs_buffers with hs_incoming_parsed = []}};
-       server_handle_client_finished_13 hs [(Finished(f),l')] []
+      //17-03-24 how to receive binders? we need the intermediate hash 
+      | S_Idle ri, ([ClientHello ch], [])  ->
+          server_handle_client_hello hs ch
 
-       | S (S_FinishedSent s), (Certificate(c),l2)::
-                   (CertificateVerify(cv),l3)::
-                   (Finished(f),l4)::[]
-         when (Some? pv && pv = Some TLS_1p3) ->
-       hsref := {!hsref with hs_buffers = {(!hsref).hs_buffers with hs_incoming_parsed = []}};
-       server_handle_client_finished_13 hs [(Finished(f),l4)] [(Certificate(c),l2);(CertificateVerify(cv),l3)]
+      | S_CCSReceived s digest, ([Finished f], [digestClientFinish]) 
+        when (Some? pv && pv <> Some TLS_1p3) -> 
+          server_ClientFinished hs f digest digestClientFinish
 
-       | C (C_Error e),_ -> InError e
-       | S (S_Error e),_ -> InError e
-       | _ , _ -> InAck false false)
+      | S_FinishedSent s, ([Finished f], [digest])
+        when (Some? pv && pv = Some TLS_1p3) -> 
+          server_ClientFinished_13 hs s f digest None 
+
+      | S_FinishedSent s, ([Certificate c; CertificateVerify cv; Finished f], [...]) 
+        when (Some? pv && pv = Some TLS_1p3) ->
+          server_ClientFinished_13 hs s f digest (Some (c,cv))  
+
+       // are we missing the case with a Certificate but no CertificateVerify? 
+
+      | C_Error e, _ -> InError e
+      | S_Error e, _ -> InError e
+      | _, _ -> InAck false false 
 
 
 val recv_ccs: s:hs -> ST incoming  // special case: CCS before 1p3; could merge with recv_fragment
@@ -1344,51 +1208,44 @@ val recv_ccs: s:hs -> ST incoming  // special case: CCS before 1p3; could merge 
     (InError? result \/ result = InAck true false)
     ))
 let recv_ccs hs =
-    let b =
-      if hs_debug then
-        IO.debug_print_string ("CALL recv_ccs\n")
-      else false in
-    let (HS #r0 r res cfg id lgref hsref) = hs in
-    let pv,kex =
-      (match (!hsref).hs_nego with
-       | None -> None, None
-       | Some n -> Some n.n_protocol_version, Some n.n_kexAlg) in
-    (match ((!hsref).hs_state,(!hsref).hs_buffers.hs_incoming_parsed) with
-    | C (C_FinishedSent n cv), [] ->
-       hsref := {!hsref with hs_buffers = {(!hsref).hs_buffers with hs_incoming_parsed = []}};
-       client_handle_server_ccs hs []
-    | C (C_FinishedSent n cv),
-      (SessionTicket(st),l)::[] ->
-       hsref := {!hsref with hs_buffers = {(!hsref).hs_buffers with hs_incoming_parsed = []}};
-       client_handle_server_ccs hs
-        [(SessionTicket(st),l)]
-    | S (S_HelloDone n),
-      (ClientKeyExchange(cke),l)::[]
-      when (Some? pv && pv <> Some TLS_1p3 &&
-            (kex = Some Kex_DHE || kex = Some Kex_ECDHE)) ->
-      hsref := {!hsref with hs_buffers = {(!hsref).hs_buffers with hs_incoming_parsed = []}};
-      server_handle_client_ccs hs
-      [(ClientKeyExchange(cke),l)] []
-    | S (S_HelloDone n),
-      (Certificate(c),l)::
-      (ClientKeyExchange(cke),l')::[]
-      when (c.crt_chain = [] && Some? pv && pv <> Some TLS_1p3 &&
-            (kex = Some Kex_DHE || kex = Some Kex_ECDHE)) ->
-      hsref := {!hsref with hs_buffers = {(!hsref).hs_buffers with hs_incoming_parsed = []}};
-      server_handle_client_ccs hs
-      [(ClientKeyExchange(cke),l')] [(Certificate(c),l)]
-    | S (S_HelloDone n),
-      (Certificate(c),l)::
-      (ClientKeyExchange(cke),l')::
-      (CertificateVerify(cv),l'')::[]
-      when (Some? pv && pv <> Some TLS_1p3 &&
-            (kex = Some Kex_DHE || kex = Some Kex_ECDHE)) ->
-      hsref := {!hsref with hs_buffers = {(!hsref).hs_buffers with hs_incoming_parsed = []}};
-      server_handle_client_ccs hs
-      [(ClientKeyExchange(cke),l')] [(Certificate(c),l);(CertificateVerify(cv),l'')]
-    | C (C_Error e),_ -> InError e
-    | S (S_Error e),_ -> InError e
-    | _,_ -> InError(AD_unexpected_message, "ClientCCS received at wrong time"))
+    IO.hs_debug_print "CALL recv_ccs\n";
+    let pv, kex = 
+      match Nego.read_mode hs.nego with // not necessarily defined early enough?
+      | Some n -> Some n.n_protocol_version, Some n.n_kexAlg
+      | None -> None, None in
+
+    // intuitively, receiving CCS triggers completion of the incoming flight of messages.
+    match Handshake.Log.ReadCCS hs.log with 
+    | Error -> InError(AD_unexpected_message, "CCS received at wrong time")
+    | Correct flight -> 
+        match !hs.state, flight with 
+        | C_FinishedSent n cv), ([], []) -> (
+            hs.state := C_CCSReceived n cv;
+            Epochs.incr_reader hs.epochs;
+            InAck true false )
+
+        | C_FinishedSent n cv, ([SessionTicket st], []) -> (
+            IO.hs_debug_print "WARNING: no support for session tickets";
+            hs.state := C_CCSReceived n cv;
+            Epochs.incr_reader hs.epochs;
+            InAck true false )
+
+        | S_HelloDone n, ([ClientKeyExchange cke], []) 
+          when (Some? pv && pv <> Some TLS_1p3 && (kex = Some Kex_DHE || kex = Some Kex_ECDHE)) ->
+            server_ClientCCS hs cke 
+(*
+        // FIXME support optional client c and cv
+        | S_HelloDone n, [Certificate c; ClientKeyExchange cke], [digestClientKeyExchange]
+          when (c.crt_chain = [] && Some? pv && pv <> Some TLS_1p3 && (kex = Some Kex_DHE || kex = Some Kex_ECDHE)) ->
+            server_ClientCCS hs cke digestClientKeyExchange (Some (c, None))
+
+        | S_HelloDone n, [Certificate c; ClientKeyExchange cke; CertificateVerify cv], [digestClientKeyExchange; digestCertificateVerify]] 
+          when (Some? pv && pv <> Some TLS_1p3 && (kex = Some Kex_DHE || kex = Some Kex_ECDHE)) ->
+            server_ClientCCS hs cke digestClientKeyExchange (Some (c, Some (cv, digestCertificateVerify)))
+*)
+        | C_Error e, _ -> InError e
+        | S_Error e, _ -> InError e
+        | _, _ -> InError(AD_unexpected_message, "CCS received at wrong time")
 
 
 val authorize: s:hs -> Cert.chain -> ST incoming // special case: explicit authorize (needed?)
